> The rest of today's notes are [handwritten](data/3.pdf) 
> Today's labs are [here](src/LambdaCalculus.hs)

# Lambda Calculus

## Basics 

Only three constructs

```hs
e ::= x       (variables)
  |   e e     (application)
  |   \x -> e (abstraction)
```

- Application associates to the left

```hs
a b c = (a b) c
```

- Only unary functions and unary application

- We usually consider terms *equal up to renaming* (alpha equivalence)
- The central computation rule is *beta reduction*

```hs
(\x -> e) (a) ->_B e [x/a]
```

**LC is important because we can encode recursion, numbers, booleans, and just about any other data type!**

## Calculation

We can calculate with:

```hs
suc := \n _> \s z -> (s (n s z))
add := \m n -> m suc n
-- Unfolded
\sz -> s^m z => suc^m n
```
We get control flow with:

```hs
true  := \tf -> t
false := \tf -> f
ifthenelse := \cte -> cte
```

`ifthenelse` is almost the identity function. We can also define `and` and `or` as follows:

```hs
and := \xy -> ifthenelse xy false
and := \xy -> x y false
or := \xy -> ifthenelse x true y
or := \xy -> x true y
```

The function `isZero` takes a number and returns a Bool.

```hs
isZero := \n -> (n (\x -> false) true)
```

## Pairs

```hs
pair := \xy -> (\p -> (p x y))

fst := \p -> (p (\xy -> x))
snd := \p -> (p (\xy -> y))
```

The function `pair` remembers its two parameters and returns them when asked by its third parameter.

```hs
fst (((\xy -> (\p -> (p xy))))) A B
-> fst (\p -> p A B)
-> (\p -> p const) (\p -> p A B)
-> \p -> const A B 
-> \p -> A
```

## Church encodings for arbitrary datatypes

There is a correspondence between the so-called *fold* (or *catamorphism* or *eliminator*) for a datatype and its Church encoding.

```hs
data Nat = Suc Nat | Zero

foldNat Zero s z    = z
foldNat (Suc n) s z = s (foldNat n s z)
```

For booleans:

```hs
data Bool = T F
foldBool :: Bool -> a -> a -> a
foldBool True  t f = t
foldBool False t f = f

true  := \xy -> x 
false := \xy -> y
```

> This is just `ifthenelse` again.

For pairs:

```hs
data Pair x y = Pair x y

foldPair (Pair x y) p = p x y
```

**The fact that we can encode certain entities in the lambda justifies that we can add them as constants to the language without changing the nature of the language.**

## Building names with `let`

`let` can simply be desugared to a lambda binding.

```hs
let x = e1 in e2 := (\x -> (e2)) e1
```

Example:

```hs
let x = BigComputation in x + x
```

Haskell has a guarantee that the `let` bound computation is only evaluated once. On the other hand, if we write:

```hs
(\x -> x + x) (BigCopmutation)
```

In non-strict languages this substitution will have `BigComputation` + `BigComputation` and it will take twice to run.


> Note that this does not work if `x` is a recursive binding or if you want to preserve sharing. 

## Recursion

```hs
fac = \n if n == 0 then 1 else n * fac (n - 1)

fac = fix
  (\fac n -> if n == 0 then 1 
                       else n * fac (n - 1))
```

The desired function `fac` can be viewed as a *fixed point* of the related non-recursive function `fac`.

A **fixed-point combinator** is a combinator fix with the property that for any `f`, 

```hs
fix :: (a -> a) -> a
-- Using recursion directly
fix f = f (fix f)
```

Here we introduce the `Y` combinator:

```hs
Y := \f -> (\x -> (f ( x x))) (\x -> (f (x x)))
```

We can now encode arbitrary recursion, `Y` has the same reduction behavior as `fix f`:

```hs
Y f -> (\x -> f (x x)) (\y -> f (y y))
    -> f ((\y -> f (y y))) (\y -> f (y y))
    -> f (Y f)
```

## General vs structural recursion

In Haskell, addition would be recursive

```hs
data Nat = Suc Nat | Zero

add (Suc m) n = Suc (add m n)
add Zero n    = n
```

- Functions defined in terms of a fold function are called *structurally recursive*.
- Recursion using the fixed-point combinator is called *general recursion*.
- Writing functions using general recursion is often perceived as simpler or more direct.
- Structural recursion is often more well-behaved. For instance, for many datatypes it can be proved that if the arguments to the fold terminate, the structurrally recursive function also rerminates.

## Pattern matching

We need to pattenr match via case on a natural number as a function:

```hs
caseNat :: Nat -> (Nat -> r) -> r -> r
caseNat (Suc n) s z = s n
caseNat Zero s z    = z

pred = \m -> caseNat m
             (\m' -> m')
            zero

foldNat :: Nat -> (s -> s) -> s -> s

caseNat n s z := 
  fst (foldNat n (\ (_, r) -> (s, r, suc r))
                              (z, zero))
```

The second component of the pair just constructs the natural number again. This is how we can access the predecessor.

### Nested patterns

```hs
fib Zero          = Zero
fib (Suc Zero)    = Suc Zero
fib (Suc (Suc n)) = add (fib n (fib (Suc n)))
```
## SKI calculus

A straightforward implementation of the LC may give rise to arbitrary large reduction steps. We can represent all lambda expressions using only three combinators with the following reduction behavior:

```hs
S f g x = (f x) (g x)
K y x  = y
I x    = x

data SKI = Var String | S | K | I | App SKI SKI

toSKI :: Lambda -> SKI
toSKI (Var x)    = x
toSKI (App 1 t2) = (toSKI t1) ` App` (toSKI t2)
toSKI (Lam x t)  = remove x (toSKI t)
```

Bracket abstraction as follows:

```hs
remove :: Var -> Lambda -> SKI
remove x (Var y)
  | x == y = I
  | otherwise K `App` y
remove x (App t1 t2) = 
  S `App` (remove (App t1 x))
    `App` (remove (App t2 x))
```

The idea behind *bracket abstraction* is that we're introducing a fake lambda using the SKI combinators. The only thing we can do with a lambda is apply it, subtitution for whatevr `\x` value is in the body. If the argument we've abstracted over is the same then we can discard the argument and keep the `K`. 

```hs
remove `x` (Var `y`)
App K (Var `y`)
```

**`S` is *duplicating* a variable; `K` is discarding a variable; `I` is using a variable.**

## More combinators

Haskell Curry proposed the following combinators:

```hs
B x y z = x (y z)
C x y z = x z y
K x y = x
W x y = x y y
```

The combinator `I` is superfluous

```hs
I := S K K x -> (K x) (K x) -> x
```

A single combinator also works!

```hs
X = \f -> (f S f3)
f3 = \p _ _ -> p  -- first of three
```

## Why care?

- GHC translates to an intermediate language: *GHC Core*.
- GHC Core is really little more than a typed lambda calculus.

## Core sketch

GHC Core is based on System Fc - a typed lambda calculus extended with type coercions.
- variables, lambdas, and application
- literals
- let bindings
- case expressions
- coercions- used to implement GADTs amongst other things
- `ticks` - used for HPC to track program coverage

Following Haskell code and corresponding Core:

```hs
f :: Int -> Int
f x = x + 1

f :: Int -> Int
f = \ (x :: Int) ->
      case x of _ { I# x1 -> I# (+# x1 1) }
```

> `#` is to deal with operatos on boxed 

